LF: Basics before Proof by Case Analysis

lf/Basics.fst
@@ -12,5 +12,338 @@
 
 // You should have received a copy of the GNU General Public License
 // along with this program.  If not, see <http://www.gnu.org/licenses/>.
-
 module Basics
+
+(** * Basics: Functional Programming in Coq *)
+
+(* REMINDER:
+
+          #####################################################
+          ###  PLEASE DO NOT DISTRIBUTE SOLUTIONS PUBLICLY  ###
+          #####################################################
+
+   (See the [Preface] for why.)
+*)
+
+(** * Introduction *)
+
+(** * Data and Functions *)
+
+(** ** Enumerated Types *)
+
+(** ** Days of the Week *)
+
+type day =
+  | Monday
+  | Tuesday
+  | Wednesday
+  | Thursday
+  | Friday
+  | Saturday
+  | Sunday
+
+val next_weekday: d: day -> Tot day
+let next_weekday = function
+    | Monday -> Tuesday
+    | Tuesday -> Wednesday
+    | Thursday -> Friday
+    | _ -> Monday
+
+val next_weekday_test: unit -> Lemma (ensures (next_weekday Friday = Monday))
+let next_weekday_test () = ()
+
+val next_weekday_test': unit -> Lemma
+  (ensures (next_weekday (next_weekday Saturday) = Tuesday))
+let next_weekday_test' () = ()
+
+(** ** Booleans *)
+
+type my_bool =
+  | T
+  | F
+
+val negb: b: my_bool -> Tot my_bool
+let negb = function
+  | T -> F
+  | F -> T
+
+val andb: b1: my_bool -> b2: my_bool -> Tot my_bool
+let andb b1 b2 =
+  match b1 with
+  | T -> b2
+  | F -> F
+
+val orb: b1: my_bool -> b2: my_bool -> Tot my_bool
+let orb b1 b2 =
+  match b1 with
+  | T -> T
+  | F -> b2
+
+val test_orb1: unit -> Lemma (ensures (orb T T = T))
+let test_orb1 () = ()
+
+val test_orb2: unit -> Lemma (ensures (orb F F = F))
+let test_orb2 () = ()
+
+val test_orb3: unit -> Lemma (ensures (orb F T = T))
+let test_orb3 () = ()
+
+val test_orb4: unit -> Lemma (ensures (orb T T = T))
+let test_orb4 () = ()
+
+(** **** Exercise: 1 star, standard (nandb)
+
+    Provide a definition of the function nandb.
+    Use the following lemmas (test_nandb1 ... test_nandb4)
+    to know about it's behavior.
+    Also fix the lemmas by replacing admit() with () and make sure
+    that they are proved *)
+
+assume val nandb: a: my_bool -> b: my_bool -> my_bool
+
+val test_nandb1: unit -> Lemma (ensures (nandb T F = T))
+let test_nandb1 () = admit()
+
+val test_nandb2: unit -> Lemma (ensures (nandb F F = T))
+let test_nandb2 () = admit()
+
+val test_nandb3: unit -> Lemma (ensures (nandb F T = T))
+let test_nandb3 () = admit()
+
+val test_nandb4: unit -> Lemma (ensures (nandb T T = F))
+let test_nandb4 () = admit()
+
+(** [] *)
+
+(** **** Exercise: 1 star, standard (andb3)
+
+    Do the same for the andb3 function below.
+    This function should return T when all of its inputs are T,
+    and F otherwise. *)
+
+assume val andb3: a: my_bool -> b: my_bool -> c: my_bool -> my_bool
+
+val test_andb31: unit -> Lemma (ensures (andb3 T T T = T))
+let test_andb31 () = admit()
+
+val test_andb32: unit -> Lemma (ensures (andb3 F T T = F))
+let test_andb32 () = admit()
+
+val test_andb33: unit -> Lemma (ensures (andb3 T F T = F))
+let test_andb33 () = admit()
+
+val test_andb34: unit -> Lemma (ensures (andb3 T T F = F))
+let test_andb34 () = admit()
+
+(** [] *)
+
+(** ** Types *)
+
+type rgb =
+  | Red
+  | Green
+  | Blue
+
+type color =
+  | Black
+  | White
+  | Primary: p: rgb -> color
+
+val isred: c: color -> Tot my_bool
+let isred = function
+  | Black -> F
+  | White -> F
+  | Primary Red -> T
+  | Primary _ -> F
+
+(** ** Tuples *)
+
+type bit =
+  | B0
+  | B1
+
+type nybble =
+  | Bits: b0: bit -> b1: bit -> b2: bit -> b3: bit -> nybble
+
+val all_zero: nb: nybble -> Tot my_bool
+let all_zero = function
+  | Bits B0 B0 B0 B0 -> T
+  | Bits _ _ _ _ -> F
+
+val all_zero_test: unit -> Lemma (ensures all_zero (Bits B1 B0 B1 B0) = F)
+let all_zero_test () = ()
+
+val all_zero_test': unit -> Lemma (ensures all_zero (Bits B0 B0 B0 B0) = T)
+let all_zero_test' () = ()
+
+(** ** Numbers *)
+
+(* Peano number (https://en.wikipedia.org/wiki/Peano_axioms) *)
+type pnat =
+  | O: pnat
+  | S: pnat -> pnat
+
+val pred: n: pnat -> Tot pnat
+let pred = function
+  | O -> O
+  | S n' -> n'
+
+val pred_test: unit -> Lemma (ensures (pred (S (S O)) = S O))
+let pred_test () = ()
+
+val minustwo: n: pnat -> Tot pnat
+let minustwo = function
+  | O -> O
+  | S O -> O
+  | S (S n') -> n'
+
+val minustwo_test: unit -> Lemma (ensures (minustwo (S (S (S (S O)))) = S (S O)))
+let minustwo_test () = ()
+
+val evenb: n: pnat -> Tot my_bool
+let rec evenb = function
+  | O -> T
+  | S O -> F
+  | S (S n') -> evenb n'
+
+val oddb: n: pnat -> Tot my_bool
+let oddb n = negb (evenb n)
+
+val test_oddb1: unit -> Lemma (ensures (oddb (S O) = T))
+let test_oddb1 () = ()
+
+val test_oddb2: unit -> Lemma (ensures (oddb (S (S (S (S O)))) = F))
+let test_oddb2 () = ()
+
+val plus: a: pnat -> b: pnat -> Tot pnat
+let rec plus a b =
+  match a with
+  | O -> b
+  | S a' -> S (plus a' b)
+
+val plus_test: unit -> Lemma
+  (ensures (plus (S (S (S O))) (S (S O)) = S (S (S (S (S O))))))
+let plus_test () = ()
+
+val mul: a: pnat -> b: pnat -> Tot pnat
+let rec mul a b =
+  match a with
+  | O -> O
+  | S a' -> plus b (mul a' b)
+
+val mul_test: unit -> Lemma
+  (ensures (mul (S (S (S O))) (S (S (S O))) = S (S (S (S (S (S (S (S (S O))))))))))
+let mul_test () = ()
+
+val minus: a: pnat -> b: pnat -> Tot pnat
+let rec minus a b =
+  match a, b with
+  | O, _ -> O
+  | S _, O -> a
+  | S a', S b' -> minus a' b'
+
+val exp: base: pnat -> power: pnat -> Tot pnat
+let rec exp base power =
+  match power with
+  | O -> S O
+  | S p -> mul base (exp base p)
+
+(** **** Exercise: 1 star, standard (factorial)
+
+    Recall the standard mathematical factorial function:
+
+       factorial(0)  =  1
+       factorial(n)  =  n * factorial(n-1)     (if n>0)
+
+   Translate it into F*.
+ *)
+
+assume val factorial: n: pnat -> pnat
+
+val test_factorial: unit -> Lemma
+  (ensures (factorial (S (S (S O))) = S (S (S (S (S (S O)))))))
+let test_factorial () = admit()
+
+(** [] *)
+
+val eqb: a: pnat -> b: pnat -> Tot my_bool
+let rec eqb a b =
+  match a, b with
+  | O, O -> T
+  | S a', S b' -> eqb a' b'
+  | _, _ -> F
+
+val leb: a: pnat -> b: pnat -> Tot my_bool
+let rec leb a b =
+  match a, b with
+  | O, _ -> T
+  | S _, O -> F
+  | S a', S b' -> leb a' b'
+
+val test_leb1: unit -> Lemma (ensures (leb (S (S O)) (S (S O)) == T))
+let test_leb1 () = ()
+
+val test_leb2: unit -> Lemma (ensures (leb (S (S O)) (S (S (S (S O)))) == T))
+let test_leb2 () = ()
+
+val test_leb3: unit -> Lemma (ensures (leb (S (S (S (S O)))) (S (S O)) == F))
+let test_leb3 () = ()
+
+(** **** Exercise: 1 star, standard (ltb)
+
+    The ltb function tests natural numbers for less-than,
+    yielding a [b]oolean.  Instead of making up a new recursive
+    definition for this one, define it in terms of a previously
+    defined function. (It can be done with just one previously defined
+    function, but you can use two if you want.) *)
+
+assume val ltb: a: pnat -> b: pnat -> my_bool
+
+val test_ltb1: unit -> Lemma (ensures (ltb (S (S O)) (S (S O)) == F))
+let test_ltb1 () = admit()
+
+val test_ltb2: unit -> Lemma (ensures (ltb (S (S O)) (S (S (S (S O)))) == T))
+let test_ltb2 () = admit()
+
+val test_ltb3: unit -> Lemma (ensures (ltb (S (S (S (S O)))) (S (S O)) == F))
+let test_ltb3 () = admit()
+
+(** [] *)
+
+(** * Proof by Simplification *)
+
+val plus_O_n: n: pnat -> Lemma (ensures (plus O n = n))
+let plus_O_n n = ()
+
+val plus_S_l: n: pnat -> Lemma (ensures (plus (S O) n = S n))
+let plus_S_l n = ()
+
+val mul_O_l: n: pnat -> Lemma (ensures (mul O n = O))
+let mul_O_l n = ()
+
+(** * Proof by Rewriting *)
+
+val plus_id_example: a: pnat -> b: pnat -> Lemma
+  (ensures (a = b ==> plus a a = plus b b))
+let plus_id_example a b = ()
+
+(** **** Exercise: 1 star, standard (plus_id_exercise)
+
+    Remove admit() and fill in the proof. *)
+val plus_id_exercise: a: pnat -> b: pnat -> c: pnat -> Lemma
+  (ensures (a = b ==> b = c ==> plus a b = plus b c))
+let plus_id_exercise a b c = admit()
+(** [] *)
+
+val mul_n_O: n: pnat -> Lemma (ensures (O = mul n O))
+let rec mul_n_O n =
+  match n with
+  | O -> ()
+  | S n' -> mul_n_O n'
+
+val mul_O_plus: n: pnat -> m: pnat -> Lemma
+  (ensures (mul (plus O n) m = mul n m))
+let rec mul_O_plus n m =
+  match n with
+  | O -> ()
+  | S n' -> mul_O_plus n' m
